theories/syntax.v
@@ -1,1 +1,5 @@
 From RichWasm.syntax Require Export modules rw.
+
+Definition primitive_rep_eq_dec (ι1 ι2 : primitive_rep) : {ι1 = ι2} + {ι1 <> ι2}.
+  decide equality.
+Defined.
